theories/Syntax/Chunks.v
@@ -39,6 +39,7 @@ From Coq Require Import
 From Katamaran Require Import
      Prelude
      Tactics
+     Syntax.Formulas
      Syntax.Predicates
      Syntax.Registers
      Base.
@@ -77,7 +78,8 @@ Qed.
 
 Module Type ChunksOn
   (Import B : Base)
-  (Import P : PredicateKit B).
+  (Import P : PredicateKit B)
+  (Import F : FormulasOn B P).
 
   (* Semi-concrete chunks *)
   Inductive SCChunk : Type :=
@@ -234,6 +236,175 @@ Module Type ChunksOn
     induction c; cbn; intros ι; f_equal; auto using peval_sound.
     apply pevals_sound. apply peval_sound.
   Qed.
+
+  Lemma inst_is_duplicable {Σ} (c : Chunk Σ) (ι : Valuation Σ) :
+    is_duplicable (inst c ι) = is_duplicable c.
+  Proof.
+    destruct c; now cbn.
+  Qed.
+
+  Section Consume.
+    Import EqNotations.
+
+    Fixpoint try_consume_chunk_exact {Σ} (h : SHeap Σ) (c : Chunk Σ) : option (SHeap Σ) :=
+      match h with
+      | nil       => None
+      | cons c' h =>
+          if chunk_eqb c c'
+          then Some (if is_duplicable c then (cons c h) else h)
+          else option_map (cons c') (try_consume_chunk_exact h c)
+      end.
+
+    Lemma try_consume_chunk_exact_spec {Σ} (h : SHeap Σ) (c : Chunk Σ) :
+      option.wlp
+        (fun h' => List.In (c , h') (heap_extractions h))
+        (try_consume_chunk_exact h c).
+    Proof.
+      induction h as [|c' h].
+      - now constructor.
+      - cbn -[is_duplicable].
+        destruct (chunk_eqb_spec c c').
+        + constructor. left. subst.
+          remember (is_duplicable c') as dup.
+          destruct dup; reflexivity.
+        + apply option.wlp_map. revert IHh.
+          apply option.wlp_monotonic; auto.
+          intros h' HIn. right.
+          rewrite List.in_map_iff.
+          exists (c,h'). auto.
+    Qed.
+
+    Section PreciseUser.
+
+      Context {Σ} (p : 𝑯) {ΔI ΔO : Ctx Ty} (prec : 𝑯_Ty p = ΔI ▻▻ ΔO)
+        (tsI : Env (Term Σ) ΔI) (tsO : Env (Term Σ) ΔO).
+
+      Equations(noeqns) match_chunk_user_precise (c : Chunk Σ) : option (PathCondition Σ) :=
+        match_chunk_user_precise (chunk_user p' ts')
+          with eq_dec p p' => {
+            match_chunk_user_precise (chunk_user ?(p) ts') (left eq_refl) :=
+              match env.catView (rew prec in ts') with
+              | env.isCat tsI' tsO' =>
+                  if env.eqb_hom Term_eqb tsI tsI'
+                  then Some (formula_eqs_ctx tsO tsO')
+                  else None
+              end;
+            match_chunk_user_precise (chunk_user p' ts') (right _) := None
+          };
+        match_chunk_user_precise _ := None.
+
+      Fixpoint find_chunk_user_precise (h : SHeap Σ) : option (SHeap Σ * PathCondition Σ) :=
+        match h with
+        | nil => None
+        | cons c h' =>
+            match match_chunk_user_precise c with
+            | Some eqs => Some (if is_duplicable p then cons c h' else h', eqs)
+            | None => option_map (base.prod_map (cons c) id) (find_chunk_user_precise h')
+            end
+        end.
+
+      Lemma find_chunk_user_precise_spec (h : SHeap Σ) :
+        option.wlp
+          (fun '(h', eqs) =>
+             forall ι : Valuation Σ,
+             instprop eqs ι ->
+             List.In
+               (inst (chunk_user p (eq_rect_r (fun c : Ctx Ty => Env (Term Σ) c) (tsI ►► tsO) prec)) ι, inst h' ι)
+               (heap_extractions (inst h ι)))
+          (find_chunk_user_precise h).
+      Proof.
+        induction h as [|c h]; [now constructor|]. cbn [find_chunk_user_precise].
+        destruct match_chunk_user_precise as [eqs|] eqn:?.
+        - clear IHh. constructor. intros ι Heqs. left.
+          destruct c; try discriminate Heqo. cbn in *.
+          destruct (eq_dec p p0); cbn in Heqo; try discriminate Heqo. destruct e.
+          remember (eq_rect (𝑯_Ty p) (Env (Term Σ)) ts (ΔI ▻▻ ΔO) prec) as ts'.
+          destruct (env.catView ts') as [tsI' tsO'].
+          destruct (env.eqb_hom_spec Term_eqb (@Term_eqb_spec Σ) tsI tsI'); try discriminate.
+          apply noConfusion_inv in Heqo. cbn in Heqo. subst.
+          apply instprop_formula_eqs_ctx in Heqs.
+          rewrite (@inst_eq_rect_indexed_r (Ctx Ty) (fun Δ Σ => Env (Term Σ) Δ) (Env Val)).
+          rewrite inst_env_cat. rewrite Heqs. rewrite <- inst_env_cat.
+          change (env.cat ?A ?B) with (env.cat A B). rewrite Heqts'.
+          rewrite (@inst_eq_rect_indexed (Ctx Ty) (fun Δ Σ => Env (Term Σ) Δ) (Env Val)).
+          rewrite rew_opp_l. now destruct is_duplicable.
+        - apply option.wlp_map. revert IHh. apply option.wlp_monotonic; auto.
+          intros [h' eqs] HYP ι Heqs. specialize (HYP ι Heqs).
+          remember (inst (chunk_user p (eq_rect_r (fun c0 : Ctx Ty => Env (Term Σ) c0) (tsI ►► tsO) prec)) ι) as c'.
+          change (inst (cons c h) ι) with (cons (inst c ι) (inst h ι)).
+          cbn [fst heap_extractions]. right. apply List.in_map_iff.
+          eexists (c', inst h' ι); auto.
+      Qed.
+
+    End PreciseUser.
+
+    Section PrecisePtsreg.
+
+      Context {Σ σ} (r : 𝑹𝑬𝑮 σ) (t : Term Σ σ).
+
+      Equations(noeqns) match_chunk_ptsreg_precise (c : Chunk Σ) : option (Formula Σ) :=
+        match_chunk_ptsreg_precise (chunk_ptsreg r' t')
+          with eq_dec_het r r' => {
+            match_chunk_ptsreg_precise (chunk_ptsreg ?(r) t') (left eq_refl) :=
+              Some (formula_relop bop.eq t t');
+            match_chunk_ptsreg_precise (chunk_ptsreg r' t') (right _) := None
+          };
+        match_chunk_ptsreg_precise _ := None.
+
+      Fixpoint find_chunk_ptsreg_precise (h : SHeap Σ) : option (SHeap Σ * PathCondition Σ) :=
+        match h with
+        | nil => None
+        | cons c h' =>
+            match match_chunk_ptsreg_precise c with
+            | Some fml => Some (h', ctx.nil ▻ fml)
+            | None => option_map (base.prod_map (cons c) id) (find_chunk_ptsreg_precise h')
+            end
+        end.
+
+      Lemma find_chunk_ptsreg_precise_spec (h : SHeap Σ) :
+        option.wlp
+          (fun '(h', eqs) =>
+             forall ι : Valuation Σ,
+             instprop eqs ι ->
+             List.In
+               (inst (chunk_ptsreg r t) ι, inst h' ι)
+               (heap_extractions (inst h ι)))
+          (find_chunk_ptsreg_precise h).
+      Proof.
+        induction h; cbn [find_chunk_ptsreg_precise]; [now constructor|].
+        destruct match_chunk_ptsreg_precise eqn:?.
+        - constructor. intros ι [Hpc Hf]. clear IHh.
+          destruct a; cbn in Heqo; try discriminate Heqo.
+          destruct (eq_dec_het r r0); try discriminate Heqo.
+          dependent elimination e. cbn in Heqo. dependent elimination Heqo.
+          change (inst (cons ?c ?h) ι) with (cons (inst c ι) (inst h ι)).
+          cbn. left. f_equal. f_equal. symmetry. exact Hf.
+        - apply option.wlp_map. revert IHh. apply option.wlp_monotonic; auto.
+          intros [h' eqs] HYP ι Heqs. specialize (HYP ι Heqs).
+          remember (inst (chunk_ptsreg r t) ι) as c'.
+          change (inst (cons ?c ?h) ι) with (cons (inst c ι) (inst h ι)).
+          cbn [fst heap_extractions]. right. apply List.in_map_iff.
+          eexists (c', inst h' ι); auto.
+      Qed.
+
+    End PrecisePtsreg.
+
+    Definition try_consume_chunk_precise {Σ} (h : SHeap Σ) (c : Chunk Σ) :
+      option (SHeap Σ * PathCondition Σ) :=
+      match c with
+      | chunk_user p ts =>
+          match 𝑯_precise p with
+          | Some (MkPrecise ΔI ΔO Δeq) =>
+              match env.catView (rew Δeq in ts) with
+              | env.isCat tsI tsO => find_chunk_user_precise Δeq tsI tsO h
+              end
+          | None => None
+          end
+      | chunk_ptsreg r t => find_chunk_ptsreg_precise r t h
+      | _ => None
+      end.
+
+  End Consume.
 
   Section Interpretation.
     Import iris.bi.interface.
